#+TITLE: Functional Programming

* References
- introduction to functional programming cite:1988-Book-Bird-Introduction

* Expression
An expression can be /reduced/ to an simpler equivalent form.  We say
an expression is /canonical/ (or in /normal form/) if it cannot be
further reduced.

The result of /equality test/ is done by reducing the expressions to
their canonical form, and testing whether the results are
identical. If an expression does not have a canonical form, the result
is undefined, represented by $\bot$. In particular, function values
have no canonical form.

The order of evaluation thus matters. Each reduction step replace a
sub-term by an equivalent term. The term is called a /redex/, short
for /reducible expression/. There are two reduction policies,
/innermost reduction/ and /outermost reduction/. /Innermost reduction/
reduces the innermost redex, i.e. the one that contains no other
redex. /Outermost reduction/ reduces the one that is contained in no
other redex.

Any term that is reduced must be reduced to /head normal form/. A term
is in /head normal form/ if it is not a redex, and it cannot become a
redex by reducing any of its subterms. For example, =(e1:e2)= is in
head normal form, because the (:) /itself/ cannot be reduced. However,
=e1= and =e2= might be reducible. It is a normal form only when e1 and
e2 both are in normal form. By definition, every term in normal form
is in head normal form, but not vice versa.

The evaluation order matters because of the /termination/. Sometimes,
the outermost reduction will terminate while the inner most fail to do
so. In fact, we have the following property:

#+begin_quote
For every term, if there exists any reduction order that terminates,
then there is an outermost reduction that terminates.
#+end_quote

Thus, outermost reduction is also called /normal order reduction/,
because it is capable of reducing a term to its normal form whenever
the term has such a form. It is also called /lazy evaluation/, because
it does not reduce a term unless it is essential for finding the
answer. By contract, the innermost reduction is called /applicative
order reduction/, or /eager evaluation/.

Outermost reduction is essential for evaluating non-strict
functions. But innermost and outermost reduction will yield the same
answer when only strict functions are involved.

With that said for termination property, however, outermost may
require more steps than innermost reduction. The reason is that, the
outermost reduction might duplicate some inner expressions. One
problem is called /graph reduction/, which ensures that the duplicated
sub-terms are always linked together in the graph, and reduction of
them will happen ones, for all the references of them. With graph
reduction, we can say outermost reduction never performs more steps
than innermost.

In summary, we shall use /outermost graph reduction/ as the evaluation
model, because
1. it terminates whenever any reduction order terminates
2. it requires no more steps than innermost order reduction

However, the outermost reduction might use more space than
innermost. In this case, it might be desired to mix innermost order to
achieve better space efficiency. There is a special function =strict=
that fine-control the evaluation order. =strict f e= is reduced by
first reducing =e= to head normal form, then applying =f=. The term
=e= itself is evaluated as normal, using outermost order. With that,
=strict= can be defined like below. We can easily have this: =f =
strict f= iff =f= is a strict function.

#+begin_example
strict f x = \bot, if x = \bot
           = f x,  otherwise
#+end_example

There are some ways to decide how to use =strict= to optimize the
space occupation, but some takeaway: for functions such as =(+)= or
=(x)=, that are strict in *both arguments*, and can be computed in
constant time and space, =foldl'= is more efficient. But for
functions, such as =(&)= and =(++)=, that are non-strict in some
argument, =foldr= is often more efficient.  (=foldl'= is a rewrite of
=foldl= with strictness)

#+begin_example
foldl' (op) a [] = a
foldl' (op) a (x:xs) = strict (foldl' (op)) (a op x) xs
#+end_example



* What is a Function?
- currying: replacing structured arguments by a sequence of simple
  ones. The function application operation associates to the left,
  i.e. =f x y= means =((f x) y)=.

** Composition
Functional composition has the definition of

$$(f \circ g) x = f (g x)$$

and the type of it

$$(\circ) :: (\beta \rightarrow \gamma) \rightarrow (\alpha
\rightarrow \beta) \rightarrow (\alpha \rightarrow \gamma)$$

functional composition is also associative, thus no need to put
brackets

$$(f \circ g) \circ h = f \circ (g \circ h)$$

** Strictness

The special value $\bot$ is polymorphic: $\bot$ is a value of every
type. This means, any function can be applied to $\bot$. If $f \bot =
\bot$, then $f$ is said to be strict. Otherwise, it is non-strict. In
other words, a function is /strict/ if it is undefined whenever its
argument is undefined.


In fact, a non-strict semantic is often preferable for functions, for
several reasons:
- it makes reasoning about equality easier
- we can define new control structures by defining new functions

For example, we define a function =three= that takes anything and
return the value =3=. I.e.

#+begin_example
three :: num -> num
three x = 3
#+end_example

Another example, the definition of =cond=

$$cond :: bool \rightarrow \alpha \rightarrow \alpha \rightarrow \alpha$$

#+begin_example
cond p x y = x, if p
           = y, otherwise
#+end_example

Under strict semantics, $cond\ True\ 0\ \bot = \bot$, under non-strict
semantics, $cond True 0 \bot = 0$. But in either case, =cond= is
strict on its first argument. This also means, strictness is bundled
with the function, and is applied on some arguments, not all.

The operational semantics of strict or non-strict functions is closely
related to the reduction strategy. /eager-evaluation/ reduces every
expression to its simplest form, while /lazy-evaluation/ does not care
about the wellness of the expressions whose values are not required
for the evaluation.

* Type
- Strong-typing: the type of an expression depends only on the type of
  its component expressions.
- Type variable: typically represented in Greek letters $\alpha$,
  $\beta$, etc. Such type can be instantiated by substitute the type
  variable with specific type.
- Polymorphic type: a type that contains /type variables/
- Enumerated type: enumeration of possible values
- Composite type: composite primitive type together to form new types
- algebraic data type: is a form of composite type, containing product
  type and sum type
  - sum type: this is like C union, so it is also called a tagged
    union. It can take value of either the type, but not both.
  - product type: this is like a C structure with different
    fields. The value set of this type is the set-theoretic product,
    i.e., the Cartesian product of the set of the field type.
- Abstract Type: types in which the values are prescribed, but the
  operations are not, are called concrete types. A type whose values
  are not defined, but operations are, is called abstract type.

** Type inference
Three basic rules

1. Application rule: if =f x :: t=, then =x :: t'= and =f :: t' -> t=
     for some new type =t'=
2. Equality rule: if both the types =x :: t= and =x :: t'= can be
     deduced for a variable =x=, then =t = t'=.
3. Function rule: If =t -> u = t' -> u'=, then =t = t'=, and =u = u'=

Often, the newly introduced types are named by numerical sub-notation.

For example, consider the composition operator

#+begin_example
(.) f g x = f (g x)
#+end_example

The following script shows the inference steps:
#+begin_example
f :: t1
g :: t2
x :: t3
f (g x) :: t4
(.) :: t1 -> t2 -> t3 -> t4
g x :: t5
f :: t5 -> t4
x :: t6
g :: t6 -> t5
t1 = t5 -> t4
t2 = t6 -> t5
t3 = t6
(.) :: (t5 -> t4) -> (t6 -> t5) -> t6 -> t4
#+end_example

Finally, we need to replace the types with type variables to make it
generic:

$$(\circ) :: (\beta \rightarrow \gamma) \rightarrow (\alpha
\rightarrow \beta) \rightarrow (\alpha \rightarrow \gamma)$$

** List
List itself is defined as a recursive type.

$$list \alpha :: Nil | Cons \alpha (list \alpha)$$


Let list comprehension notation be =[<expr> | <qualifier>;
...]=. Qualifier can be boolean expression for predicates or
generators. Later generators vary more quickly than their
predecessors, and can depends on the variables introduced by earlier
ones. With this, we can define many operators on lists:

#+begin_example
(++) :: [a] -> [a] -> [a]
concat :: [[a]] -> [a]
concat xss = [x | xs <- xss; x <- xs]
#+end_example

Instead of using =(++)= for concating list, we can use =(:)=
(pronounced 'cons') for specifying consing. One important reason to
use =(:)= is that, every list can be expressed in terms of =[]= and
=(:)= in *exactly one way*.

#+begin_example
(:) :: a -> [a] -> [a]
x:xs = [x] ++ xs
#+end_example

We have the following operators on lists:
#+begin_example

(#) :: [a] -> num
#(xs ++ ys) = #xs + #ys

hd :: [a] -> a
tl :: [a] -> [a]
hd ([x] ++ xs) = x
tl ([x] ++ xs) = xs

take n xs ++ drop n xs = xs

takewhile :: (a -> bool) -> [a]  -> [a]
zip :: ([a], [b]) -> [(a,b)]
(!) :: [a] -> num -> a # index

#+end_example

Map and filter can be defined by:
#+begin_example
map :: (a -> b) -> [a] -> [b]
map f xs = [f x | x <- xs]
filter :: (a -> bool) -> [a] -> [a]
filter p xs = [x | x <- xs; p x]
#+end_example

Fold:
#+begin_example
foldr :: (a -> b -> b) -> b -> [a] -> b
foldl :: (b -> a -> b) -> b -> [a] -> b
sum = foldr (+) 0
product = foldr (x) 1
concat = foldr (++) []
and = foldr (&) True
or = foldr (|) False
#+end_example

=foldr= and =foldl= do rely on associative of the underlying operators
to function correctly, and there are several /duality theorems/.

In big data literature, /map/ and /reduce/ are borrowed from
functional programming. Map is just map, reduce has another familiar
name called /fold/.  The Map-reduce framework does not just borrow the
name. Its contribution is *scalability and fault-tolerance*. In this
case, /map/ produces data by filtering, and emit the data,
marshalling, and /reduce/ does folding.

* Recursion

Functions are often defined recursively. In this section, we see some
of the list function definitions in recursion.

#+begin_example
zip([], ys) = []
zip(x:xs, []) = []
zip(x:xs, y:ys) = (x,y):zip(xs,ys)
#+end_example

#+begin_example
take 0 xs = []
take (n+1) [] = []
take (n+1) (x:xs) = x:take n xs

drop 0 xs = xs
drop (n+1) [] = []
drop (n+1) (x:xs) = drop n xs
#+end_example

#+begin_example
hd(x:xs) = x
tl(x:xs) = xs
#+end_example

#+begin_example
map f [] = []
map f (x:xs) = f x : map f xs
filter p [] = []
filter p (x:xs) = x : filter p xs, if p x
                = filter p xs,     otherwise
#+end_example

bibliography:../../research/bib/manual/book.bib
